Soundness updated with spawn blocks

SporkProofs/Inline.lean
@@ -1,5 +1,9 @@
 import SporkProofs.Syntax
 import SporkProofs.Semantics
+import SporkProofs.WFSyntax
+import SporkProofs.WFSemantics
+
+abbrev x := Nat
 
 structure Extra where
   offset : Nat
@@ -10,20 +14,22 @@ structure Extra where
 namespace Extra
   @[simp] def add (bsig : BlockSig) (extra : Extra) : BlockSig :=
     ⟨bsig.Γ + extra.Γ, extra.r, bsig.σ ++ extra.σ⟩
+  @[simp] def spork (extra : Extra) (r : Nat) : Extra :=
+    Extra.mk extra.offset 0 r []
   theorem add_spork_comm {bsig : BlockSig} {extra : Extra} {s : Nat} :
                          (extra.add bsig).spork s = extra.add (bsig.spork s) :=
-    by simp
+    by simp; exact ⟨rfl, rfl⟩
 end Extra
 
 @[simp] def inlinedArgs (extra : Extra) (scope : Nat) (args : List Var) : List Var :=
   args ++ (List.range' scope extra.Γ).map Var.mk
 
 @[simp] def inlinedCont (extra : Extra) (scope : Nat) : Cont -> Cont
-  | .mk b args => .mk (b + extra.offset) (inlinedArgs extra scope args)
+  | .mk b args => .mk (b + extra.offset) (inlinedArgs extra scope args)  
 
-@[simp] def inlinedCode (bret : BlockIdx) (extra : Extra) (scope : Nat) : Code -> Code
+@[simp] def inlinedCode (B: List BlockSig) (bret : BlockIdx) (extra : Extra) (scope : Nat) : Code -> Code
   | .stmt e c =>
-    .stmt e (inlinedCode bret extra scope.succ c)
+    .stmt e (inlinedCode B bret extra scope.succ c)
   | .goto bnext =>
     .goto (inlinedCont extra scope bnext)
   | .ite cond bthen belse =>
@@ -35,17 +41,17 @@ end Extra
   | .retn args =>
     .goto (.mk bret (inlinedArgs extra scope args))
   | .spork bbody bspwn =>
-    .spork (inlinedCont extra scope bbody) (inlinedCont extra scope bspwn)
+    .spork (inlinedCont extra scope bbody) (inlinedCont (extra.spork B[bspwn.b]!.r) scope bspwn)
   | .spoin bunpr bprom =>
     .spoin (inlinedCont extra scope bunpr)
            (inlinedCont extra scope bprom)
 
-@[simp] def inlinedBlock (bret : BlockIdx) (extra : Extra) (b : Block) : Block :=
-  Block.mk (extra.add b.bsig) (inlinedCode bret extra b.bsig.Γ b.code)
+@[simp] def inlinedBlock (B : List BlockSig) (bret : BlockIdx) (extra : Extra) (b : Block) : Block :=
+  Block.mk (extra.add b.bsig) (inlinedCode B bret extra b.bsig.Γ b.code)
 
 theorem inlinedArgsRangeWF :
     (extraArity : Nat) -> (scope : Nat) ->
-    IVec (·.WF (scope + extraArity)) ((List.range' scope extraArity).map Var.mk)
+    IVec ((scope + extraArity) ⊢ · WF-var) ((List.range' scope extraArity).map Var.mk)
   | 0, scope => .nil
   | .succ extraArity, scope =>
     .cons (.mk (by simp))
@@ -54,23 +60,19 @@ theorem inlinedArgsRangeWF :
            inlinedArgsRangeWF extraArity scope.succ)
 
 theorem inlinedArgsWF' (extra : Extra) {scope : Nat} : {args : List Var} ->
-                       IVec (·.WF scope) args -> IVec (·.WF (scope + extra.Γ)) args
-  | [], .nil => .nil
-  | _a :: _args, .cons awf argswf =>
-    .cons (Var.WF.mk (Nat.lt_add_right extra.Γ awf.idx))
-          (inlinedArgsWF' extra argswf)
+                       IVec (scope ⊢ · WF-var) args -> IVec ((scope + extra.Γ) ⊢ · WF-var) args
+  | _args, wf => wf.weaken
 
 theorem inlinedArgsWF (extra : Extra) {scope : Nat} {args : List Var}
-                      (wf : IVec (·.WF scope) args) :
-                      IVec (·.WF (scope + extra.Γ)) (inlinedArgs extra scope args) :=
+                      (wf : IVec (scope ⊢ · WF-var) args) :
+                      IVec ((scope + extra.Γ) ⊢ · WF-var) (inlinedArgs extra scope args) :=
   (inlinedArgsWF' extra wf).append (inlinedArgsRangeWF extra.Γ scope)
 
 theorem inlinedContWFRets
         {bsigs bsigs' bsig rets} (extra : Extra) {c : Cont}
         (bslen : bsigs.length = extra.offset)
-        (wf : c.WFRets bsigs' bsig rets) :
-        (inlinedCont extra bsig.Γ c).WFRets
-          (bsigs ++ bsigs'.map extra.add) (extra.add bsig) rets :=
+        (wf : bsigs'; bsig ⊢ c(rets) WF-cont) :
+        (bsigs ++ bsigs'.map extra.add); (extra.add bsig) ⊢ (inlinedCont extra bsig.Γ c)(rets) WF-cont :=
   .mk (by simp[← bslen, Nat.add_comm c.b bsigs.length, wf.blt])
       (by simp[wf.bsig, Nat.add_comm c.b extra.offset, ← bslen]
           rw[Nat.add_assoc, Nat.add_comm rets extra.Γ, ← Nat.add_assoc])
@@ -79,41 +81,30 @@ theorem inlinedContWFRets
 theorem inlinedContWF
         {bsigs bsigs' bsig} (extra : Extra) {c : Cont}
         (bslen : bsigs.length = extra.offset)
-        (wf : c.WF bsigs' bsig) :
-        (inlinedCont extra bsig.Γ c).WF
-          (bsigs ++ bsigs'.map extra.add) (extra.add bsig) :=
+        (wf : bsigs'; bsig ⊢ c WF-cont) :
+        (bsigs ++ bsigs'.map extra.add); (extra.add bsig) ⊢ (inlinedCont extra bsig.Γ c) WF-cont :=
   (inlinedContWFRets extra bslen wf.cast0).cast0
-
-theorem inlinedAtomWF {Γ : Nat} (extraArity : Nat) : {a : Atom} -> a.WF Γ -> a.WF (Γ + extraArity)
-  | .val _v, _wf => .val
-  | .var _v, wf => .var (.mk (Nat.lt_add_right extraArity wf.vwf.idx))
-
-theorem inlinedExprWF {Γ : Nat} (extraArity : Nat) : {e : Expr} -> e.WF Γ -> e.WF (Γ + extraArity)
-  | .nop _a, .nop awf =>
-    .nop (inlinedAtomWF extraArity awf)
-  | .uop _o _a, .uop awf =>
-    .uop (inlinedAtomWF extraArity awf)
-  | .bop _o _a _b, .bop awf bwf =>
-    .bop (inlinedAtomWF extraArity awf) (inlinedAtomWF extraArity bwf)
 
 theorem inlinedCodeWF
     {fsigs bsigs bsigs' bsig bret}
     (bretlt : bret < bsigs.length)
     (extra : Extra)
-    (bretsig : bsigs[bret] = ⟨bsig.r + extra.Γ, extra.r, extra.σ⟩)
+    (bretsig : bsigs[bret] = ⟨bsig.r + extra.Γ, bsig.r, extra.σ⟩)
+--    (bretsig : (bsigs[bret].Γ = bsig.r + extra.Γ) ∧ (bsigs[bret].r = bsig.r) ∧ (bsigs[bret].σ = extra.σ))
     (bslen : bsigs.length = extra.offset) :
     {c : Code} ->
-    c.WF fsigs bsigs' bsig ->
-    (inlinedCode bret extra bsig.Γ c).WF
-      fsigs (bsigs ++ bsigs'.map extra.add) (extra.add bsig)
+    fsigs; bsigs'; bsig ⊢ c WF-code ->
+    fsigs; (bsigs ++ bsigs'.map extra.add); (extra.add bsig) ⊢
+      (inlinedCode bsigs bret extra bsig.Γ c) WF-code
   | .stmt e c, wf =>
-    .stmt (inlinedExprWF extra.Γ wf.stmt_expr)
+    .stmt wf.stmt_expr.weaken
           (by simpa[Nat.add_right_comm bsig.Γ extra.Γ 1]
-              using inlinedCodeWF (bsig := bsig.bind) bretlt extra bretsig bslen (wf.stmt_code))
+              using inlinedCodeWF (bsig := bsig.bind) bretlt extra
+                                  bretsig bslen (wf.stmt_code))
   | .goto bnext, wf =>
     .goto (inlinedContWF extra bslen wf.goto_bnext)
   | .ite cond bthen belse, wf =>
-    .ite (inlinedAtomWF extra.Γ wf.ite_cond)
+    .ite wf.ite_cond.weaken
          (inlinedContWF extra bslen wf.ite_bthen)
          (inlinedContWF extra bslen wf.ite_belse)
   | .call h args bret', wf =>
@@ -123,9 +114,12 @@ theorem inlinedCodeWF
           (inlinedContWFRets extra bslen wf.call_bret)
   | .retn args, .retn len sn_nil argswf =>
     .goto (.mk (by simp[Nat.lt_add_right bsigs'.length bretlt])
-               (by rw[List.getElem_append_left (bs := bsigs'.map extra.add) bretlt]
+               (by simp only [getters]
+                   rw[List.getElem_append_left (bs := bsigs'.map extra.add) bretlt]
                    simp[sn_nil]
-                   rw[← len, ← bretsig])
+                   rw[← len, bretsig]
+                   simp
+                   exact sorry)
                (inlinedArgsWF extra argswf))
   | .spork bbody bspwn, wf =>
     .spork (Extra.add_spork_comm ▸
@@ -142,48 +136,64 @@ theorem inlinedCodeWF
                              (bsigs'.length_map extra.add ▸ wf.spork_bspwn.blt)).r =
                           bsigs'[bspwn.b]!.r :=
                     List.getElem_map extra.add ▸
-                    congrArg (·.r) bretsig ▸
-                    sorry
+                    --congrArg (·.r) bretsig ▸
+                    by simp
                   rw[h]
                   exact wf.spork_bbody))
-           (inlinedContWF extra bslen wf.spork_bspwn)
+           (--(bsigs ++ List.map (fun bsig => Extra.add bsig extra) bsigs')[(inlinedCont extra bsig.Γ bspwn).b]!
+            by
+              let iclt : (inlinedCont extra bsig.Γ bspwn).b < bsigs.length :=
+                sorry
+              let l : (bsigs ++ List.map (fun bsig => Extra.add bsig extra) bsigs')[(inlinedCont extra bsig.Γ bspwn).b]! = bsigs[(inlinedCont extra bsig.Γ bspwn).b]! :=
+                by rw[getElem!_pos (bsigs ++ bsigs'.map extra.add) (inlinedCont extra bsig.Γ bspwn).b (by simp at iclt ⊢; exact Nat.lt_add_right bsigs'.length iclt)]
+                   rw[List.getElem_append_left (as := bsigs) (bs := bsigs'.map extra.add) (i := (inlinedCont extra bsig.Γ bspwn).b) iclt]
+                   symm
+                   exact getElem!_pos bsigs (inlinedCont extra bsig.Γ bspwn).b iclt
+              rw[getElem!_pos bsigs (inlinedCont extra bsig.Γ bspwn).b iclt] at l
+              rw[l]
+              let bspwn' := inlinedContWF (extra.spork bsigs[(inlinedCont extra bsig.Γ bspwn).b].r) bslen wf.spork_bspwn
+              simpa using bspwn')
     -- .spork wf.spork_flt
     --        wf.spork_arity
     --        (inlinedArgsWF' extra wf.spork_args)
     --        (inlinedContWF extra bslen wf.spork_bbody)
   | .spoin bunpr bprom, wf =>
-    .spoin (by simp[wf.spoin_sn_nonnil])
-           (by simp[List.tail_append_of_ne_nil wf.spoin_sn_nonnil]
+    .spoin (λ x => by simp at x; exact wf.spoin_oblg x.1)
+           (by simp[List.tail_append_of_ne_nil wf.spoin_oblg]
                exact inlinedContWF extra bslen wf.spoin_bunpr)
-           (by simp[List.tail_append_of_ne_nil wf.spoin_sn_nonnil,
-                    List.head_append_left wf.spoin_sn_nonnil]
+           (by simp[List.tail_append_of_ne_nil wf.spoin_oblg,
+                    List.head_append_left wf.spoin_oblg]
                exact inlinedContWFRets extra bslen wf.spoin_bprom)
 
+l
+
 theorem inlinedBlockWF
-    {fsigs bsigs bsigs' ret ret' bret}
+    {fsigs bsigs bsigs' bret}
     (bretlt : bret < bsigs.length)
     (extra : Extra)
-    (bretsig : bsigs[bret] = ⟨ret + extra.bsig.Γ, extra.bsig.sporkNest⟩)
     (bslen : bsigs.length = extra.offset)
     {b : Block}
-    (wf : b.WF fsigs bsigs' ret) :
-    (inlinedBlock bret extra b).WF
-      fsigs (bsigs ++ bsigs'.map (· + extra.bsig)) ret' :=
-  .mk (inlinedCodeWF bretlt extra bretsig bslen wf.1)
+    (bretsig : (bsigs[bret].Γ ≤ b.bsig.Γ + extra.Γ) ∧ (bsigs[bret].σ = extra.σ))
+--    (bretsig : bsigs[bret] = ⟨b.bsig.r + extra.Γ, extra.r, extra.σ⟩)
+    (wf : fsigs; bsigs' ⊢ b WF-block) :
+    fsigs; (bsigs ++ bsigs'.map extra.add) ⊢ (inlinedBlock bsigs bret extra b) WF-block :=
+  .mk (inlinedCodeWF bsigs bretlt extra bretsig bslen wf.1)
 
-@[simp] def inlinedFuncBody (g : Func) (bret : Cont) (sporks : Oblg) (offset : Nat) : List Block :=
-  g.blocks.map (inlinedBlock bret.b (.mk offset (.mk bret.args.length sporks)))
+@[simp] def inlinedFuncBody (g : Func) (bret : Cont) (σ : List Nat) (offset : Nat) : List Block :=
+  g.blocks.map (inlinedBlock bret.b (.mk offset bret.args.length σ))
 
 theorem inlinedFuncBodyWF
-          {fsigs bsigs ret g bret sporks}
+          {fsigs bsigs ret g bret σ}
           (bretlt : bret.b < bsigs.length)
-          (bretsig : bsigs[bret.b] = ⟨g.fsig.ret + bret.args.length, sporks⟩)
-          (wf : g.WF fsigs) :
-          IVec (·.WF fsigs (bsigs ++ List.map (· + .mk bret.args.length sporks) g.bsigs) ret)
-               (inlinedFuncBody g bret sporks bsigs.length) :=
+          (bretsig : bsigs[bret.b] = ⟨bret.args.length, ret, σ⟩)
+          (wf : fsigs ⊢ g WF-func) :
+          IVec (fsigs; (bsigs ++ g.B.map (Extra.mk bsigs.length bret.args.length σ).add) ⊢ · WF-block)
+               (inlinedFuncBody g bret σ bsigs.length) :=
   wf.blocks.from_map'
-    (inlinedBlock bret.b (.mk bsigs.length (.mk bret.args.length sporks)))
-    (λ _b => inlinedBlockWF bretlt (.mk bsigs.length (.mk bret.args.length sporks)) bretsig rfl)
+    (inlinedBlock bret.b (.mk bsigs.length bret.args.length σ))
+    (λ _b => inlinedBlockWF bretlt (.mk bsigs.length bret.args.length σ) rfl
+               ⟨congrArg BlockSig.Γ bretsig ▸ by simp,
+                congrArg BlockSig.σ bretsig⟩)
 
 @[simp] def replaceCallInCode (g : FuncIdx) (offset : Nat) (c : Code) : Option (Code × Cont) :=
   let (e, ⟨t, _p⟩) := c.split
@@ -206,18 +216,18 @@ theorem inlinedFuncBodyWF
         (.mk bsig c, [])
         (λ (c', bret) =>
           (.mk bsig c',
-           inlinedFuncBody g bret bsig.sporkNest
+           inlinedFuncBody g bret bsig.σ
              (bacc ++ [Block.mk bsig c'] ++ bs ++ gacc).length))
     inlinedFuncH g gidx (bacc ++ [b']) bs (gacc ++ gacc')
 
 theorem inlinedFuncHWF
         {fsigs fsig g gidx bacc gacc} :
         {bs : List Block} ->
-        g.WF fsigs ->
+        fsigs ⊢ g WF-func ->
         (_ : gidx < fsigs.length) ->
         fsigs[gidx] = g.fsig ->
-        (Func.mk fsig (bacc ++ bs ++ gacc)).WF fsigs ->
-        (Func.mk fsig (inlinedFuncH g gidx bacc bs gacc)).WF fsigs
+        fsigs ⊢ Func.mk fsig (bacc ++ bs ++ gacc) WF-func ->
+        fsigs ⊢ Func.mk fsig (inlinedFuncH g gidx bacc bs gacc) WF-func
   | [], gwf, glt, gsig, wf => List.append_nil bacc ▸ wf
   | .mk bsig c :: bs, gwf, glt, gsig, wf => by
     simp
@@ -237,7 +247,7 @@ theorem inlinedFuncHWF
             let c' : Code :=
               .merge es (.goto (.mk (bacc.length + (bs.length + gacc.length + 1))
                                    (args ++ bret.args)))
-            let gacc' := inlinedFuncBody g bret bsig.sporkNest
+            let gacc' := inlinedFuncBody g bret bsig.σ
                            (bacc ++ [Block.mk bsig c'] ++ bs ++ gacc).length
             let bsigs := (bacc ++ Block.mk bsig c' :: bs ++ gacc ++ gacc').map (·.bsig)
             let wf' := wf.blocks.get ⟨bacc.length, by simp⟩
@@ -245,32 +255,33 @@ theorem inlinedFuncHWF
             let cwf := wf'.code
             let splitwf := Code.WF.split_wf cwf
             simp[cspliteq] at splitwf
-            let c'wf : c'.WF fsigs bsigs fsig.ret bsig := by
+            let c'wf : fsigs; bsigs; bsig ⊢ c' WF-code := by
               simp[c', bsigs]
               apply Code.WF.merge_wf
               · exact λ ⟨i, il⟩ => splitwf.1 ⟨i, by simp_all⟩
-              · apply Code.WF.goto; apply Cont.WF.mk <;> simp
+              · apply Code.WF.goto
+                apply Cont.WF.mk <;> simp
                 · simp[gacc']
                   let gh := gwf.head.get0eq
                   simp at gh; rw[gh]; simp
-                  show g.fsig.arity = args.length
-                  exact gsig ▸ splitwf.2.call_arity
+                  --show g.fsig.arity = args.length
+                  --exact gsig ▸ splitwf.2.call_arity
+                  exact gsig ▸ ⟨splitwf.2.call_arity, sorry, rfl⟩ 
                 · exact splitwf.2.call_args.append splitwf.2.call_bret.args
                 · match gacc'eq : gacc' with
                     | [] => simp[gacc'] at gacc'eq
                             let ghead := gwf.head.headtail
                             simp[gacc'eq] at ghead
                     | _ :: _ => simp
-            let b'wf : (Block.mk bsig c').WF fsigs bsigs fsig.ret := .mk c'wf
+            let b'wf : fsigs; bsigs ⊢ ⟨bsig, c'⟩ WF-block := .mk c'wf
             let wfblocks := wf.blocks
             let ⟨tmp, gaccwf⟩ := wf.blocks.unappend
             let ⟨baccwf, tmp'⟩ := tmp.unappend
             let bswf := tmp'.tail
-            let helper {l : List Block} (v : IVec (Block.WF fsigs (List.map (fun x => x.bsig) (Func.mk fsig (bacc ++ Block.mk bsig c :: bs ++ gacc)).blocks) (Func.mk fsig (bacc ++ Block.mk bsig c :: bs ++ gacc)).fsig.ret) l) : IVec (Block.WF fsigs (List.map (fun x => x.bsig) (Func.mk fsig (bacc ++ [Block.mk bsig c'] ++ bs ++ (gacc ++ gacc'))).blocks) (Func.mk fsig (bacc ++ [Block.mk bsig c'] ++ bs ++ (gacc ++ gacc'))).fsig.ret) l :=
-              v.map (λ b x => by simpa using x.weaken_bsigs (bsigs' := gacc'.map (·.bsig)))
-            let wf'' : Func.WF fsigs (.mk fsig (bacc ++ [.mk bsig c'] ++ bs
-                                                  ++ (gacc ++ gacc'))) := by
-              apply Func.WF.mk
+            let helper {l : List Block} (v : IVec (fsigs; ((bacc ++ Block.mk bsig c :: bs ++ gacc).map Block.bsig) ⊢ · WF-block) l) : IVec (Block.WF fsigs ((bacc ++ [Block.mk bsig c'] ++ bs ++ (gacc ++ gacc')).map Block.bsig)) l :=
+              v.map (λ b x => by simpa using x.weaken_B (B' := gacc'.map (·.bsig)))
+            let wf'' : fsigs ⊢ ⟨fsig, bacc ++ [.mk bsig c'] ++ bs ++ (gacc ++ gacc')⟩ WF-func := by
+              apply Blocks.WF.mk
               · apply IVec.append
                 · apply IVec.append
                   · apply IVec.append
@@ -280,7 +291,12 @@ theorem inlinedFuncHWF
                   · exact helper bswf
                 · apply IVec.append
                   · exact helper gaccwf
-                  · simp[gacc']; let x := @inlinedFuncBodyWF fsigs ((bacc ++ [Block.mk bsig c'] ++ bs ++ gacc).map (·.bsig)) fsig.ret g bret bsig.sporkNest (by simpa using splitwf.2.call_bret.blt) (by simpa[gsig, Nat.add_comm] using splitwf.2.call_bret.bsig) gwf; simp at x; exact x
+                  · simp[gacc']; let x := @inlinedFuncBodyWF fsigs ((bacc ++ [Block.mk bsig c'] ++ bs ++ gacc).map (·.bsig)) ((bacc.map Block.bsig ++ bsig :: (bs.map Block.bsig ++ gacc.map Block.bsig))[bret.b]'sorry).r g bret bsig.σ (by simpa using splitwf.2.call_bret.blt)
+                      --(by simpa[gsig, Nat.add_comm] using splitwf.2.call_bret.bsig)
+                      (by simp[gsig, Nat.add_comm];
+                          rw[splitwf.2.call_bret.bsig]
+                          exact sorry)
+                      gwf; simp at x; exact x
               · cases bacc <;> simp <;> simp at wf <;>
                 apply HeadIs.mk <;> simpa using wf.head.get0eq
             simpa[c', gacc']
@@ -294,9 +310,9 @@ def inlinedFunc (f g : Func) (gidx : FuncIdx) : Func :=
   .mk f.fsig (inlinedFuncH g gidx [] f.blocks [])
 
 theorem inlinedFuncWF {fsigs} {f g : Func} {gidx : FuncIdx}
-                      (gwf : g.WF fsigs) (glt : gidx < fsigs.length)
-                      (gsig : fsigs[gidx] = g.fsig) (wf : f.WF fsigs) :
-                      (inlinedFunc f g gidx).WF fsigs :=
+                      (gwf : fsigs ⊢ g WF-func) (glt : gidx < fsigs.length)
+                      (gsig : fsigs[gidx] = g.fsig) (wf : fsigs ⊢ f WF-func) :
+                      fsigs ⊢ inlinedFunc f g gidx WF-func :=
   inlinedFuncHWF gwf glt gsig ((List.append_nil f.blocks).symm ▸ wf)
 
 namespace Program
