SporkProofs/WFSemantics.lean
@@ -104,15 +104,19 @@ namespace SpawnDeque
     | mk (_ : IVec (B ⊢ · WF-spawn) ρ.unpr) (_: SpawnOrder canProm ρ.prom)
 
   namespace WF
-    notation (name := notationwf) B:arg "; " canProm:arg " ⊢ " ρ:arg " WF-deque" => WF B canProm ρ
+    notation (name := notationwf) B:arg "; " canProm:arg " ⊢ " ρ " WF-deque" => WF B canProm ρ
   
     instance {B canProm} : (ρ : SpawnDeque) -> Decidable (B; canProm ⊢ ρ WF-deque)
       | .mk u p => decidable_of_iff
           (IVec (B ⊢ · WF-spawn) u ∧ SpawnOrder canProm p)
           ⟨λ ⟨a, b⟩ => ⟨a, b⟩, λ ⟨a, b⟩ => ⟨a, b⟩⟩
     
-    theorem unpr {fsigs canProm} {ρ : SpawnDeque} : fsigs; canProm ⊢ ρ WF-deque -> IVec (fsigs ⊢ · WF-spawn) ρ.unpr | mk u _p => u
-    theorem prom {fsigs canProm} {ρ : SpawnDeque} : fsigs; canProm ⊢ ρ WF-deque -> SpawnOrder canProm ρ.prom | mk _u p => p
+    theorem unpr {B canProm ρ} : B; canProm ⊢ ρ WF-deque -> IVec (B ⊢ · WF-spawn) ρ.unpr | mk u _p => u
+    theorem prom {B canProm ρ} : B; canProm ⊢ ρ WF-deque -> SpawnOrder canProm ρ.prom | mk _u p => p
+    theorem push {B canProm ρ bspwn} (ρwf : B; canProm ⊢ ρ WF-deque) (bspwnwf : B ⊢ bspwn WF-spawn) : B; canProm ⊢ ρ.push bspwn WF-deque :=
+      ⟨ρwf.1.concat bspwnwf, ρwf.2⟩
+    theorem unpush {B canProm ρ bspwn} (ρwf : B; canProm ⊢ ρ.push bspwn WF-deque) : B; canProm ⊢ ρ WF-deque :=
+      ⟨ρwf.1.unconcat.1, ρwf.2⟩
 
     theorem castCanProm {fsigs ρ} : {canProm : Bool} -> (canProm' : Bool) -> canProm ≤ canProm' -> fsigs; canProm ⊢ ρ WF-deque -> fsigs; canProm' ⊢ ρ WF-deque
       | false, false, _, .mk MatchesOblg p => .mk MatchesOblg p
@@ -162,66 +166,72 @@ namespace SpawnDeque
 end SpawnDeque
 
 namespace StackFrame
-  inductive WF (P : Program) (K : CallStack) (gets : Nat) : StackFrame -> Prop where
+  inductive WF (P : Program) (K : CallStack) (get : Nat) : StackFrame -> Prop where
     | mk {f ρ X b} :
          (flt : f < P.size) ->
          (blt : b < P[f].B.length) ->
-         (P[f].B[b].Γ ≤ X.length + gets ∧ P[f].B[b].σ = ρ.sig P[f].B) ->
-         --P[f].B[b] = ⟨X.length + gets, P[f].B[b].r, ρ.sig P[f].B⟩ ->
+         (P[f].B[b].Γ ≤ X.length + get ∧ P[f].B[b].σ = ρ.sig P[f].B) ->
+         --P[f].B[b] = ⟨X.length + get, P[f].B[b].r, ρ.sig P[f].B⟩ ->
          P[f].B; K.allPromoted ⊢ ρ WF-deque ->
-         (mk f ρ X b).WF P K gets
+         (mk f ρ X b).WF P K get
 
   namespace WF
-    notation (name := notationwf) P:arg "; " K:arg "; " gets:arg " ⊢ " k " WF-frame" => WF P K gets k
+    notation (name := notationwf) P:arg "; " K:arg "; " get:arg " ⊢ " k " WF-frame" => WF P K get k
     notation (name := notationwf') P:arg "; " K:arg " ⊢ " k " WF-frame" => WF P K 0 k
-    instance {P K gets} : (k : StackFrame) -> Decidable (P; K; gets ⊢ k WF-frame)
+    instance {P K get} : (k : StackFrame) -> Decidable (P; K; get ⊢ k WF-frame)
       | .mk f ρ X b =>
         decidable_of_iff (∃ flt : f < P.size,
                           ∃ blt : b < P[f].B.length,
-                          --P[f].B[b] = ⟨X.length + gets, P[f].B[b].r, ρ.sig P[f].B⟩ ∧
-                          (P[f].B[b].Γ ≤ X.length + gets ∧ P[f].B[b].σ = ρ.sig P[f].B) ∧
+                          --P[f].B[b] = ⟨X.length + get, P[f].B[b].r, ρ.sig P[f].B⟩ ∧
+                          (P[f].B[b].Γ ≤ X.length + get ∧ P[f].B[b].σ = ρ.sig P[f].B) ∧
                           P[f].B; K.allPromoted ⊢ ρ WF-deque)
           ⟨λ ⟨a, b, c, d⟩ => ⟨a, b, c, d⟩, λ ⟨a, b, c, d⟩ => ⟨a, b, c, d⟩⟩
 
-    theorem flt {P K gets} : {k : StackFrame} ->
-                P; K; gets ⊢ k WF-frame -> k.f < P.size
+    theorem flt {P K get} : {k : StackFrame} ->
+                P; K; get ⊢ k WF-frame -> k.f < P.size
       | .mk _f _ρ _X _b, mk flt _blt _bsig _ρwf => flt
 
-    theorem blt {P K gets} : {k : StackFrame} ->
-                (wf : P; K; gets ⊢ k WF-frame) -> k.b < (P[k.f]'wf.flt).B.length
+    theorem blt {P K get} : {k : StackFrame} ->
+                (wf : P; K; get ⊢ k WF-frame) -> k.b < (P[k.f]'wf.flt).B.length
       | .mk _f _ρ _X _b, mk _flt blt _bsig _ρwf => blt
 
-    theorem blt' {P K gets k} (wf : P; K; gets ⊢ k WF-frame) :
+    theorem blt' {P K get k} (wf : P; K; get ⊢ k WF-frame) :
                  k.b < (P[k.f]'wf.flt).size :=
       (P[k.f]'wf.flt).size_eq_B_length ▸ wf.blt
 
-    theorem ρwf {P K gets} : {k : StackFrame} ->
-                (wf : P; K; gets ⊢ k WF-frame) -> (P[k.f]'wf.flt).B; K.allPromoted ⊢ k.ρ WF-deque
+    theorem ρwf {P K get} : {k : StackFrame} ->
+                (wf : P; K; get ⊢ k WF-frame) -> (P[k.f]'wf.flt).B; K.allPromoted ⊢ k.ρ WF-deque
       | .mk _f _ρ _X _b, mk _flt _blt _bsig ρwf => ρwf
 
-    theorem bsig {P K gets} : {k : StackFrame} ->
-                 (wf : P; K; gets ⊢ k WF-frame) ->
-                 (((P[k.f]'wf.flt).B[k.b]'wf.blt).Γ ≤ k.X.length + gets ∧
+    theorem bsig {P K get} : {k : StackFrame} ->
+                 (wf : P; K; get ⊢ k WF-frame) ->
+                 (((P[k.f]'wf.flt).B[k.b]'wf.blt).Γ ≤ k.X.length + get ∧
                   ((P[k.f]'wf.flt).B[k.b]'wf.blt).σ = k.ρ.sig (P[k.f]'wf.flt).B)
-                 -- ((P[k.f]'wf.flt).B[k.b]'wf.blt) = ⟨k.X.length + gets, ((P[k.f]'wf.flt).B[k.b]'wf.blt).r, k.ρ.sig (P[k.f]'wf.flt).B⟩
+                 -- ((P[k.f]'wf.flt).B[k.b]'wf.blt) = ⟨k.X.length + get, ((P[k.f]'wf.flt).B[k.b]'wf.blt).r, k.ρ.sig (P[k.f]'wf.flt).B⟩
       | .mk _f _ρ _X _b, mk _flt _blt bsig _ρwf => bsig
 
-    theorem bsig! {P K gets} : {k : StackFrame} ->
-                 (wf : P; K; gets ⊢ k WF-frame) ->
-                 (P[k.f]!.B[k.b]!.Γ ≤ k.X.length + gets ∧
+    theorem bsig! {P K get} : {k : StackFrame} ->
+                 (wf : P; K; get ⊢ k WF-frame) ->
+                 (P[k.f]!.B[k.b]!.Γ ≤ k.X.length + get ∧
                   P[k.f]!.B[k.b]!.σ = k.ρ.sig P[k.f]!.B)
---                 P[k.f]!.B[k.b]! = ⟨k.X.length + gets, P[k.f]!.B[k.b]!.r, k.ρ.sig P[k.f]!.B⟩
+--                 P[k.f]!.B[k.b]! = ⟨k.X.length + get, P[k.f]!.B[k.b]!.r, k.ρ.sig P[k.f]!.B⟩
       | .mk f _ρ _X b, mk flt blt bsig _ρwf =>
         getElem!_pos P f flt ▸
         getElem!_pos P[f].B b blt ▸
         bsig
 
-    theorem changeStack {P K K' gets k} :
-                        P; K; gets ⊢ k WF-frame ->
+    theorem changeStack {P K K' get k} :
+                        P; K; get ⊢ k WF-frame ->
                         (K.allPromoted ≤ K'.allPromoted) ->
-                        P; K'; gets ⊢ k WF-frame
+                        P; K'; get ⊢ k WF-frame
       | .mk flt blt bsig ρwf, klt =>
         .mk flt blt bsig (ρwf.castCanProm K'.allPromoted klt)
+
+    theorem promote {P K get f bspwn u p X b} (kprom : K.allPromoted) :
+                    P; K; get ⊢ ⟨f, ⟨bspwn :: u, p⟩, X, b⟩ WF-frame ->
+                    P; K; get ⊢ ⟨f, ⟨u, bspwn :: p⟩, X, b⟩ WF-frame
+      | .mk flt blt bsig ρwf =>
+        .mk flt blt bsig (kprom ▸ (kprom ▸ ρwf).promote)
 
     theorem spawn {P f bspwn} (flt : f < P.size) (bwf : P[f].B ⊢ bspwn WF-spawn) :
                   P; .nil ⊢ .spawn f bspwn WF-frame :=
@@ -258,6 +268,23 @@ namespace StackFrame
         (bnext_wf : P[f].B; ⟨X.length, P[f].B[bnext.b]!.r, ρ.sig P[f].B⟩ ⊢ bnext WF-cont) :
         P; K ⊢ ⟨f, ρ, X[bnext.args]'bnext_wf.args, bnext.b⟩ WF-frame :=
       goto_rets p ρwf bnext_wf
+
+    theorem goto_rets!
+        {P} {f K ρ} {X : ValMap} {bnext : Cont} {r : Nat}
+        (flt : f < P.size)
+        (ρwf : P[f].B; K.allPromoted ⊢ ρ WF-deque)
+        (bnext_wf : P[f].B; ⟨X.length, P[f].B[bnext.b]!.r, ρ.sig P[f].B⟩ ⊢ bnext(r) WF-cont) :
+        P; K; r ⊢ ⟨f, ρ, X[bnext.args]!, bnext.b⟩ WF-frame :=
+      getElem!_pos X bnext.args bnext_wf.args ▸
+      goto_rets flt ρwf bnext_wf
+
+    theorem goto!
+        {P} {f K ρ} {X : ValMap} {bnext : Cont}
+        (flt : f < P.size)
+        (ρwf : P[f].B; K.allPromoted ⊢ ρ WF-deque)
+        (bnext_wf : P[f].B; ⟨X.length, P[f].B[bnext.b]!.r, ρ.sig P[f].B⟩ ⊢ bnext WF-cont) :
+        P; K ⊢ ⟨f, ρ, X[bnext.args]!, bnext.b⟩ WF-frame :=
+      goto_rets! flt ρwf bnext_wf
   
     theorem goto_entry
         {P} (Pwf : P WF-program) {f K} {X : ValMap} {x : List Var}
@@ -268,25 +295,38 @@ namespace StackFrame
       entry Pwf p (xwf.map_length (λ x xwf => X[x]) ▸ sigwf)
   end WF
 
-  @[simp] def ret {P K gets} (k : StackFrame) (kwf : P; K; gets ⊢ k WF-frame) : Nat :=
+  @[simp] def ret {P K get} (k : StackFrame) (kwf : P; K; get ⊢ k WF-frame) : Nat :=
     ((P[k.f]'kwf.flt).B[k.b]'kwf.blt).r
 
   @[simp] def ret! (P : Program) (k : StackFrame) : Nat :=
     P[k.f]!.B[k.b]!.r
 
-  @[simp] def code {P K gets} (k : StackFrame) (kwf : P; K; gets ⊢ k WF-frame) : Code :=
+  @[simp] def code {P K get} (k : StackFrame) (kwf : P; K; get ⊢ k WF-frame) : Code :=
     ((P[k.f]'kwf.flt)[k.b]'kwf.blt').code
 
+  @[simp] def bsig! (P : Program) (k : StackFrame) : BlockSig :=
+    ⟨k.X.length, P[k.f]!.B[k.b]!.r, k.ρ.sig P[k.f]!.B⟩
+  @[simp] def bsig {P K get} (k : StackFrame) (wf : P; K; get ⊢ k WF-frame) : BlockSig :=
+    let flt := wf.flt
+    let blt := wf.blt
+    ⟨k.X.length, (P[k.f].B[k.b]).r, k.ρ.sig P[k.f].B⟩
+
   namespace WF
-    @[simp] theorem ret!_eq_ret {P K k gets} (kwf : P; K; gets ⊢ k WF-frame) : k.ret! P = k.ret kwf :=
+    theorem ret!_eq_ret {P K k get} (kwf : P; K; get ⊢ k WF-frame) : k.ret! P = k.ret kwf :=
       by rw[ret, ret!,
             getElem!_pos P k.f kwf.flt,
             getElem!_pos (P[k.f]'kwf.flt).B k.b kwf.blt]
 
-    @[simp] theorem code!_eq_code {P K k gets} (kwf : P; K; gets ⊢ k WF-frame) : k.code! P = k.code kwf :=
+    theorem code!_eq_code {P K k get} (kwf : P; K; get ⊢ k WF-frame) : k.code! P = k.code kwf :=
       by rw[code, code!,
             getElem!_pos P k.f kwf.flt,
             getElem!_pos (P[k.f]'kwf.flt) k.b kwf.blt']
+
+    theorem bsig!_eq_bsig {P K get} : {k : StackFrame} -> (wf : P; K; get ⊢ k WF-frame) -> k.bsig wf = k.bsig! P
+      | ⟨f, _ρ, _X, b⟩, wf =>
+        by simp only [StackFrame.bsig, getters, StackFrame.bsig!]
+           rw[getElem!_pos P f wf.flt,
+              getElem!_pos (P[f]'wf.flt).B b wf.blt]
   end WF
 end StackFrame
 
@@ -294,33 +334,33 @@ end StackFrame
 namespace CallStack
 
   /--
-  (Potentially partial) call stack, awaiting a return of `gets` args.
-  When `gets` is `none`, this must be a full call stack,
+  (Potentially partial) call stack, awaiting a return of `get` args.
+  When `get` is `none`, this must be a full call stack,
   where the current frame is at the surface of the stack.
-  When `gets` is `some n`, it is a partial call stack awaiting
+  When `get` is `some n`, it is a partial call stack awaiting
   a return of `n` args from the following stack frame
   -/
-  inductive WF (P : Program) : (gets : Option Nat) -> CallStack -> Prop where
-    | nil {gets : Nat} : nil.WF P (some gets)
-    | cons {K k} {gets : Option Nat} :
-           P; K; (gets.getD 0) ⊢ k WF-frame ->
+  inductive WF (P : Program) : (get : Option Nat) -> CallStack -> Prop where
+    | nil {get : Nat} : nil.WF P (some get)
+    | cons {K k} {get : Option Nat} :
+           P; K; (get.getD 0) ⊢ k WF-frame ->
            K.WF P (some (k.ret! P)) ->
-           (K ⬝ k).WF P gets
+           (K ⬝ k).WF P get
 
   namespace WF
     notation (name := callstackwfcons) t " ⬝wf " h:arg => WF.cons h t
-    notation (name := notationwf) P:arg "; " gets:arg " ⊢ " K:arg " WF-stack" => WF P gets K
+    notation (name := notationwf) P:arg "; " get:arg " ⊢ " K " WF-stack" => WF P get K
     notation (name := notationwf') P:arg " ⊢ " K " WF-stack" => WF P none K
 
-    instance instDecidable {P} : {gets : Option Nat} -> (K : CallStack) ->
-                           Decidable (P; gets ⊢ K WF-stack)
-      | some gets, .nil => isTrue .nil
+    instance instDecidable {P} : {get : Option Nat} -> (K : CallStack) ->
+                           Decidable (P; get ⊢ K WF-stack)
+      | some get, .nil => isTrue .nil
       | none, .nil => isFalse (λ _ => by contradiction)
-      | gets, K ⬝ k =>
+      | get, K ⬝ k =>
         let _ : Decidable (P; (k.ret! P) ⊢ K WF-stack) := instDecidable K
-        decidable_of_iff (P; K; (gets.getD 0) ⊢ k WF-frame ∧ K.WF P (some (k.ret! P)))
+        decidable_of_iff (P; K; (get.getD 0) ⊢ k WF-frame ∧ K.WF P (some (k.ret! P)))
           ⟨λ ⟨a, b⟩ => .cons a b, λ | .cons a b => ⟨a, b⟩⟩
-        -- dite (P; K; (gets.getD 0) ⊢ k WF-frame)
+        -- dite (P; K; (get.getD 0) ⊢ k WF-frame)
         --   (λ kwf => let _ : Decidable (P; (k.ret kwf) ⊢ K WF-stack) :=
         --               instDecidable K
         --             decidable_of_iff (P; (k.ret kwf) ⊢ K WF-stack)
@@ -329,30 +369,30 @@ namespace CallStack
 
     theorem nonnil {P} {K : CallStack} (Kwf : P ⊢ K WF-stack) : K ≠ CallStack.nil :=
       by cases Kwf <;> simp
-    theorem head' {P gets} :
+    theorem head' {P get} :
                   {K : CallStack} ->
                   (nn : K ≠ CallStack.nil) ->
-                  P; gets ⊢ K WF-stack ->
-                  P; K.tail; (gets.getD 0) ⊢ (K.head nn) WF-frame
+                  P; get ⊢ K WF-stack ->
+                  P; K.tail; (get.getD 0) ⊢ (K.head nn) WF-frame
       | _K ⬝ _k, _nn, _Kwf ⬝wf kwf => kwf
-    theorem tail' {P gets} :
+    theorem tail' {P get} :
                   {K : CallStack} ->
                   (nn : K ≠ CallStack.nil) ->
-                  (Kwf : P; gets ⊢ K WF-stack) ->
+                  (Kwf : P; get ⊢ K WF-stack) ->
                   P; (some ((K.head nn).ret! P)) ⊢ K.tail WF-stack
       | _K ⬝ _k, _nn, Kwf ⬝wf _kwf => Kwf
-    theorem head! {P gets} :
+    theorem head! {P get} :
                   {K : CallStack} ->
                   (nn : K ≠ CallStack.nil) ->
-                  P; gets ⊢ K WF-stack ->
-                  P; K.tail; (gets.getD 0) ⊢ K.head! WF-frame
+                  P; get ⊢ K WF-stack ->
+                  P; K.tail; (get.getD 0) ⊢ K.head! WF-frame
       | _K ⬝ _k, _nn, _Kwf ⬝wf kwf => kwf
 
-    theorem head {P gets K k} (Kwf : P; gets ⊢ (K ⬝ k) WF-stack) :
-                 P; K; (gets.getD 0) ⊢ k WF-frame :=
+    theorem head {P get K k} (Kwf : P; get ⊢ (K ⬝ k) WF-stack) :
+                 P; K; (get.getD 0) ⊢ k WF-frame :=
       head' (by simp) Kwf
 
-    theorem tail {P gets K k} (Kwf : P; gets ⊢ (K ⬝ k) WF-stack) :
+    theorem tail {P get K k} (Kwf : P; get ⊢ (K ⬝ k) WF-stack) :
                  P; (some (k.ret! P)) ⊢ K WF-stack :=
       tail' (by simp) Kwf
 
@@ -380,27 +420,9 @@ namespace CallStack
       retjoin_eq_retjoin?! (K := K ⬝ k) wf.tail
 
   @[simp] def bsig! (P : Program) (K : CallStack) : BlockSig :=
-    ⟨K.head!.X.length,
-     (P[K.head!.f]!.B[K.head!.b]!).r,
-     K.head!.ρ.sig P[K.head!.f]!.B⟩
+    K.head!.bsig! P
   @[simp] def bsig {P : Program} (K : CallStack) (wf : P ⊢ K WF-stack) : BlockSig :=
-    let flt := wf.current.flt
-    let blt := wf.current.blt
-    ⟨(K.head wf.nonnil).X.length,
-     (P[(K.head wf.nonnil).f].B[(K.head wf.nonnil).b]).r,
-     (K.head wf.nonnil).ρ.sig P[(K.head wf.nonnil).f].B⟩
-  @[simp] def bsig' {P : Program} : (K : CallStack) -> (wf : P ⊢ K WF-stack) -> BlockSig
-    | K ⬝ ⟨f, ρ, X, b⟩, wf =>
-      let flt := wf.current.flt
-      let blt := wf.current.blt
-      ⟨X.length, P[f].B[b].r, ρ.sig P[f].B⟩
-  theorem bsig_eq_bsig' {P : Program} : {K : CallStack} -> (wf : P ⊢ K WF-stack) -> K.bsig wf = K.bsig' wf
-    | _K ⬝ ⟨_f, _ρ, _X, _b⟩, _wf => rfl
-  theorem bsig!_eq_bsig {P : Program} : {K : CallStack} -> (wf : P ⊢ K WF-stack) -> K.bsig wf = K.bsig! P
-    | _K ⬝ ⟨f, _ρ, _X, b⟩, wf =>
-      by simp only [bsig, getters, bsig!]
-         rw[getElem!_pos P f wf.current.flt,
-            getElem!_pos (P[f]'wf.current.flt).B b wf.current.blt]
+    (K.head wf.nonnil).bsig wf.current
 
   -- @[simp] def code! (P : Program) (K : CallStack) : Code :=
   --   K.head!.code! P
@@ -408,14 +430,14 @@ namespace CallStack
     (K.head wf.nonnil).code wf.current
 
   namespace WF
-    theorem append {P} : {K K' : CallStack} -> {gets : Option Nat} ->
-                   P; (some (K'.retjoin P)) ⊢ K WF-stack -> P; gets ⊢ K' WF-stack ->
-                   K' ≠ .nil -> K.allPromoted -> P; gets ⊢ (K ++ K') WF-stack
-      | K, .nil ⬝ k, gets, Kwf, K'wf@(.nil ⬝wf kwf), _knn, kprom =>
+    theorem append {P} : {K K' : CallStack} -> {get : Option Nat} ->
+                   P; (some (K'.retjoin P)) ⊢ K WF-stack -> P; get ⊢ K' WF-stack ->
+                   K' ≠ .nil -> K.allPromoted -> P; get ⊢ (K ++ K') WF-stack
+      | K, .nil ⬝ k, get, Kwf, K'wf@(.nil ⬝wf kwf), _knn, kprom =>
         by simp; exact
           (Option.some_inj.mp (retjoin_eq_retjoin?! K'wf) ▸ Kwf) ⬝wf
           (kwf.changeStack (λ _ => kprom))
-      | K, K' ⬝ k' ⬝ k, gets, Kwf, K'wf ⬝wf kwf, p, kprom =>
+      | K, K' ⬝ k' ⬝ k, get, Kwf, K'wf ⬝wf kwf, p, kprom =>
         (append Kwf K'wf (λ x => by contradiction) kprom) ⬝wf
           (kwf.changeStack (by simp[← ·, allPromoted_iff_nil.mp kprom]))
 
@@ -440,6 +462,49 @@ namespace CallStack
         let k'wf : P; (K' ⬝ k'); (get.getD 0) ⊢ k WF-frame :=
           wf.head.changeStack (λ kap => by simp at kap; simp[kap])
         ⟨Kwf, K'wf ⬝wf k'wf⟩
+        
+
+      @[simp] def peeph_retjoin? (P : Program) : CallStack -> Option Nat
+          | .nil => none
+          | .nil ⬝ k => some P[k.f]!.B[k.b]!.r
+          | K ⬝ _k => peeph_retjoin? P K
+      @[simp] theorem peeph_retjoin?_eq {P : Program} {K : CallStack} : (peeph_retjoin? P K).getD 0 = K.retjoin P :=
+        by induction K
+           · case nil => rfl
+           · case cons K k ih =>
+             cases K
+             · case nil => rfl
+             · case cons K k' => simpa using ih
+      @[simp] theorem peeph_cons_isSome {P K k} : (peeph_retjoin? P (K ⬝ k)).isSome = true :=
+        by induction K generalizing k
+           · case nil => rfl
+           · case cons K' k' ih => exact ih
+
+    theorem peep {P K k K'} (wf : P ⊢ (K ⬝ k ++ K') WF-stack) :
+                 P; K; (K'.retjoin P) ⊢ k WF-frame := by
+      rw[← append_one, append_assoc] at wf
+      let rec h : (K' : CallStack) -> (get : Option Nat) ->
+                  P; get ⊢ (K ++ ({k} ++ K')) WF-stack ->
+                  P; K; (((peeph_retjoin? P K') <|> get).getD 0) ⊢ k WF-frame
+        | .nil, a, wf => wf.head
+        | .nil ⬝ k'', get, wf => by simpa using wf.tail.head
+        | K'' ⬝ k'' ⬝ k''', get, wf =>
+          let hk := h (K'' ⬝ k'') (some (StackFrame.ret! P k''')) (wf.tail)
+          by rw[peeph_retjoin?,
+                Option.orElse_eq_orElse,
+                ← Option.or_eq_orElse,
+                Option.or_of_isSome peeph_cons_isSome]
+             · rw[Option.orElse_eq_orElse,
+                  ← Option.or_eq_orElse,
+                  Option.or_of_isSome peeph_cons_isSome] at hk
+               exact hk
+             · exact CallStack.noConfusion
+      simpa using h K' none wf
+
+    theorem bsig!_eq_bsig {P K} (wf : P ⊢ K WF-stack) : K.bsig wf = K.bsig! P := by
+      simp only [bsig!, bsig]
+      rw[wf.current.bsig!_eq_bsig,
+         CallStack.head!_eq_head wf.nonnil]
 
     theorem code!_eq_code {P : Program} {K : CallStack} (Kwf : P ⊢ K WF-stack) : K.code! P = K.code Kwf :=
       by rw[CallStack.code!,
@@ -457,7 +522,7 @@ namespace CallStack
           by simpa using kwf.blt
         let Xlen : (P[k.f].B[k.b]'kwf.blt).Γ ≤ k.X.length :=
           by simpa only [Option.getD_none, Nat.add_zero] using kwf.bsig.1
-        by simp only [getters, CallStack.code, StackFrame.code, CallStack.bsig]
+        by simp only [getters, CallStack.code, StackFrame.code, CallStack.bsig, StackFrame.bsig]
            rw[← kwf.bsig.2,
               ← Nat.add_sub_of_le Xlen]
            simpa using Pwf⁅k.f⁆⁅k.b⁆.code.weaken_Γ
@@ -474,6 +539,14 @@ namespace CallStack
                   (flt : f < P.size) (bwf : P[f].B ⊢ bspwn WF-spawn) :
                   P ⊢ spawn f bspwn WF-stack :=
       .nil ⬝wf (.spawn flt bwf)
+
+    theorem promote {P get K f bspwn u p X b} (kprom : K.allPromoted) : {K' : CallStack} ->
+                    P; get ⊢ K ⬝ ⟨f, ⟨bspwn :: u, p⟩, X, b⟩ ++ K' WF-stack ->
+                    P; get ⊢ K ⬝ ⟨f, ⟨u, bspwn :: p⟩, X, b⟩ ++ K' WF-stack
+      | .nil, Kwf ⬝wf kwf =>
+        Kwf ⬝wf (kwf.promote kprom)
+      | K' ⬝ k', K'wf ⬝wf k'wf =>
+        promote kprom K'wf ⬝wf (k'wf.changeStack (λ x => by simp at x))
   end WF
 end CallStack
 
@@ -496,7 +569,7 @@ namespace Thread
               P.fsigs; (P[(T.K.head wf.K.nonnil).f]'wf.K.current.flt).B; (T.K.bsig wf.K) ⊢ T.c WF-code :=
       getElem!_pos P (T.K.head wf.K.nonnil).f wf.K.current.flt ▸
       T.K.head!_eq_head wf.K.nonnil ▸
-      T.K.bsig!_eq_bsig wf.K ▸
+      wf.K.bsig!_eq_bsig ▸
       wf.c!
 
     theorem nonnil {P} {T : Thread} (wf : P ⊢ T WF-thread) : T.K ≠ .nil := wf.K.nonnil
@@ -542,6 +615,15 @@ namespace Thread
     theorem spawn {P f bspwn} (Pwf : P WF-program) (flt : f < P.size) (bwf : P[f].B ⊢ bspwn WF-spawn) :
                   P ⊢ spawn P f bspwn flt bwf WF-thread :=
       fromStack Pwf (.spawn flt bwf)
+
+    theorem promote {P K f bspwn u p X b K' c} (kprom : K.allPromoted)
+                    (wf : P ⊢ (K ⬝ ⟨f, ⟨bspwn :: u, p⟩, X, b⟩ ++ K') ⋄ c WF-thread) :
+                    P ⊢ (K ⬝ ⟨f, ⟨u, bspwn :: p⟩, X, b⟩ ++ K') ⋄ c WF-thread :=
+      .mk (wf.K.promote kprom)
+          (let wfc := wf.c
+           by cases K' <;>
+              (rw[← getElem!_pos P, ← CallStack.head!_eq_head,
+                  CallStack.WF.bsig!_eq_bsig] at wfc; exact wfc))
   end WF
 end Thread
 
