SporkProofs/Soundness.lean
@@ -5,38 +5,38 @@ import SporkProofs.Preservation
 
 namespace Steps
 
-  theorem preservation {P : Program} (Pwf : P.WF) :
+  theorem preservation {P : Program} (Pwf : P WF-program) :
                         {R R' : ThreadTree} ->
-                        R.WF P -> P ⊢ R ↦* R' -> R'.WF P
+                        P ⊢ R WF-tree -> P ⊢ R ↦* R' -> P ⊢ R' WF-tree
     | R, .(R), Rwf, .nil => Rwf
     | R, R'', Rwf, @Steps.cons .(P) .(R) R' .(R'') R_sR' R'_R'' =>
       Step.preservation Pwf (preservation Pwf Rwf R_sR') R'_R''
 
-  theorem preserves_prom {P : Program} (Pwf : P.WF) : {R R' : ThreadTree} ->
-                         P ⊢ R ↦* R' -> R.WF P -> R.prom = R'.prom
+  theorem preserves_prom {P : Program} (Pwf : P WF-program) : {R R' : ThreadTree} ->
+                         P ⊢ R ↦* R' -> P ⊢ R WF-tree -> R.prom = R'.prom
   | R, .(R), .nil, _Rwf  => rfl
   | R, R'', @Steps.cons .(P) .(R) R' .(R'') R_R' R'_R'', Rwf =>
     let p_R_R' : R.prom = R'.prom := preserves_prom Pwf R_R' Rwf
     let p_R'_R'' : R'.prom = R''.prom := Step.preserve_prom R'_R'' (preservation Pwf Rwf R_R')
     Eq.trans p_R_R' p_R'_R''
 
-  def soundness {P : Program} (Pwf : P.WF) {R R' : ThreadTree}
-                (Rwf : R.WF P) (R_R' : P ⊢ R ↦* R') : Step.Next P R' :=
+  def soundness {P : Program} (Pwf : P WF-program) {R R' : ThreadTree}
+                (Rwf : P ⊢ R WF-tree) (R_R' : P ⊢ R ↦* R') : Step.Next P R' :=
     Step.progress R' (preservation Pwf Rwf R_R')
 
   inductive NextRoot (P : Program) : ThreadTree -> Type where
-    | result (g X x) :
-        NextRoot P {{⟨g, ∅, X, .code (.retn x)⟩}}
+    | result (g X b x) :
+        NextRoot P {{⟨g, ∅, X, b⟩} ⋄ .retn x}
     | step {R} (R') (s : P ⊢ R ↦ R') :
         NextRoot P R
 
-  def program_soundness {P : Program} (Pwf : P.WF) {R : ThreadTree}
-                        (ss : P ⊢ (ThreadTree.init P) ↦* R) : NextRoot P R :=
+  def program_soundness {P : Program} (Pwf : P WF-program) {R : ThreadTree}
+                        (ss : P ⊢ (ThreadTree.init P Pwf) ↦* R) : NextRoot P R :=
     let Piwf := ThreadTree.WF.init Pwf
     let Rwf := preservation Pwf Piwf ss
     match Step.progress R Rwf with
-      | .result g X x => .result g X x
-      | .blocked K f gret π X bunpr bprom =>
+      | .result g X b x => .result g X b x
+      | .blocked K f bspwn π X b bunpr bprom =>
         let c := preserves_prom Pwf ss Piwf
         by contradiction
       | .step R' s => .step R' s
